Build the theories in CI

Soundness.thy
@@ -2,65 +2,65 @@ theory Soundness
   imports Defs
 begin
 
-lemma context_invariance: "⟦ Γ ⊢ e : τ ; ∀x τ'. atom x ∈ fv_term e ∧ (x, τ') ∈ Γ ⟶ (x, τ') ∈ Γ' ⟧ ⟹ Γ' ⊢ e : τ"
-proof(nominal_induct Γ e τ avoiding: Γ' rule: T.strong_induct)
-  case (T_UnitI Γ)
+lemma context_invariance: "\<lbrakk> \<Gamma> \<turnstile> e : \<tau> ; \<forall>x \<tau>'. atom x \<in> fv_term e \<and> (x, \<tau>') \<in> \<Gamma> \<longrightarrow> (x, \<tau>') \<in> \<Gamma>' \<rbrakk> \<Longrightarrow> \<Gamma>' \<turnstile> e : \<tau>"
+proof(nominal_induct \<Gamma> e \<tau> avoiding: \<Gamma>' rule: T.strong_induct)
+  case (T_UnitI \<Gamma>)
   then show ?case using T.T_UnitI by simp
 next
-  case (T_VarI x τ Γ)
+  case (T_VarI x \<tau> \<Gamma>)
   then show ?case using T.T_VarI supp_at_base by fastforce
 next
-  case (T_AbsI x Γ τ1 e τ2)
+  case (T_AbsI x \<Gamma> \<tau>1 e \<tau>2)
   then show ?case using T.T_AbsI by fastforce
 next
-  case (T_AppI Γ e1 τ1 τ2 e2)
+  case (T_AppI \<Gamma> e1 \<tau>1 \<tau>2 e2)
   then show ?case by (metis T.T_AppI Un_iff term.fv_defs(3))
 next
-  case (T_LetI x Γ e1 τ1 e2 τ2)
-  then have 1: "atom x ♯ (Γ', e1)" by simp
-  from T_LetI have 2: "(x, τ1) # Γ' ⊢ e2 : τ2" by simp
+  case (T_LetI x \<Gamma> e1 \<tau>1 e2 \<tau>2)
+  then have 1: "atom x \<sharp> (\<Gamma>', e1)" by simp
+  from T_LetI have 2: "(x, \<tau>1) # \<Gamma>' \<turnstile> e2 : \<tau>2" by simp
   show ?case using T.T_LetI[OF 1 2] using T_LetI by simp
 qed
 
-lemma free_in_context: "⟦ Γ ⊢ e : τ ; atom x ∈ fv_term e ⟧ ⟹ ∃τ'. (x, τ') ∈ Γ"
-proof(nominal_induct Γ e τ avoiding: x rule: T.strong_induct)
-  case (T_UnitI Γ)
+lemma free_in_context: "\<lbrakk> \<Gamma> \<turnstile> e : \<tau> ; atom x \<in> fv_term e \<rbrakk> \<Longrightarrow> \<exists>\<tau>'. (x, \<tau>') \<in> \<Gamma>"
+proof(nominal_induct \<Gamma> e \<tau> avoiding: x rule: T.strong_induct)
+  case (T_UnitI \<Gamma>)
   then show ?case by simp
 next
-  case (T_VarI x' τ Γ)
+  case (T_VarI x' \<tau> \<Gamma>)
   then show ?case by (metis atom_eq_iff singletonD supp_at_base term.fv_defs(1))
 next
-  case (T_AbsI x' Γ τ1 e τ2)
+  case (T_AbsI x' \<Gamma> \<tau>1 e \<tau>2)
   then show ?case by (metis Diff_iff Un_iff fresh_def insert_iff isin.simps(2) list.set(2) no_vars_in_ty term.fv_defs(2))
 next
-  case (T_AppI Γ e1 τ1 τ2 e2)
+  case (T_AppI \<Gamma> e1 \<tau>1 \<tau>2 e2)
   then show ?case by auto
 next
-  case (T_LetI x' Γ e1 τ1 e2 τ2)
+  case (T_LetI x' \<Gamma> e1 \<tau>1 e2 \<tau>2)
   then show ?case by (metis Diff_iff UnE fresh_at_base(2) isin.simps(2) term.fv_defs(5))
 qed
 
-lemma fresh_term[simp]: "⟦ Γ ⊢ e : τ ; atom x ♯ Γ ⟧ ⟹ atom x ♯ e"
-  apply (nominal_induct Γ e τ avoiding: x rule: T.strong_induct)
+lemma fresh_term[simp]: "\<lbrakk> \<Gamma> \<turnstile> e : \<tau> ; atom x \<sharp> \<Gamma> \<rbrakk> \<Longrightarrow> atom x \<sharp> e"
+  apply (nominal_induct \<Gamma> e \<tau> avoiding: x rule: T.strong_induct)
       apply (auto simp: fresh_Cons)
   using fresh_ineq_at_base fresh_not_isin apply force
   done
 
-lemma fun_ty_lam: "⟦ Γ ⊢ e : τ1 → τ2 ; is_v_of_e e ⟧ ⟹ ∃x e'. e = (λx:τ1. e')"
-  by (nominal_induct Γ e "τ1 → τ2" rule: T.strong_induct) auto
+lemma fun_ty_lam: "\<lbrakk> \<Gamma> \<turnstile> e : \<tau>1 \<rightarrow> \<tau>2 ; is_v_of_e e \<rbrakk> \<Longrightarrow> \<exists>x e'. e = (\<lambda>x:\<tau>1. e')"
+  by (nominal_induct \<Gamma> e "\<tau>1 \<rightarrow> \<tau>2" rule: T.strong_induct) auto
 
-theorem progress: "[] ⊢ e : τ ⟹ is_v_of_e e ∨ (∃e'. Step e e')"
-proof (induction "[] :: Γ" e τ rule: T.induct)
+theorem progress: "[] \<turnstile> e : \<tau> \<Longrightarrow> is_v_of_e e \<or> (\<exists>e'. Step e e')"
+proof (induction "[] :: \<Gamma>" e \<tau> rule: T.induct)
   case T_UnitI
   then show ?case by simp
 next
-  case (T_VarI x τ)
+  case (T_VarI x \<tau>)
   then show ?case by simp
 next
-  case (T_AbsI x τ1 e τ2)
+  case (T_AbsI x \<tau>1 e \<tau>2)
   then show ?case by simp
 next
-  case (T_AppI e1 τ1 τ2 e2)
+  case (T_AppI e1 \<tau>1 \<tau>2 e2)
   note IH1 = T_AppI(2)
   note IH2 = T_AppI(4)
 
@@ -70,103 +70,103 @@ next
     from IH2 show ?thesis
     proof (elim disjE)
       assume "is_v_of_e e2"
-      from ‹is_v_of_e e1› T_AppI(1) have "∃x e. e1 = (λx:τ1. e)" by (simp add: fun_ty_lam)
-      then have "∃e'. Step (App e1 e2) e'" using ‹is_v_of_e e2› ST_BetaI by blast
+      from \<open>is_v_of_e e1\<close> T_AppI(1) have "\<exists>x e. e1 = (\<lambda>x:\<tau>1. e)" by (simp add: fun_ty_lam)
+      then have "\<exists>e'. Step (App e1 e2) e'" using \<open>is_v_of_e e2\<close> ST_BetaI by blast
       then show ?thesis by simp
     next
-      assume "∃e2'. Step e2 e2'"
-      then show ?thesis using ST_App2I ‹is_v_of_e e1› by blast
+      assume "\<exists>e2'. Step e2 e2'"
+      then show ?thesis using ST_App2I \<open>is_v_of_e e1\<close> by blast
     qed
   next
-    assume "∃e1'. Step e1 e1'"
+    assume "\<exists>e1'. Step e1 e1'"
     then obtain e1' where "Step e1 e1'" by blast
     then have "Step (App e1 e2) (App e1' e2)" by (rule ST_AppI)
     then show ?thesis by blast
   qed
 next
-  case (T_LetI e1 τ1 x e2 τ2)
+  case (T_LetI e1 \<tau>1 x e2 \<tau>2)
   then show ?case using ST_SubstI ST_LetI by blast
 qed
 
-lemma swap_term: "⟦ Γ ⊢ e : τ ; atom y ♯ Γ ⟧ ⟹ ((x ↔ y) ∙ Γ) ⊢ (x ↔ y) ∙ e : τ"
-proof (nominal_induct Γ e τ avoiding: x y rule: T.strong_induct)
-  case (T_UnitI Γ)
+lemma swap_term: "\<lbrakk> \<Gamma> \<turnstile> e : \<tau> ; atom y \<sharp> \<Gamma> \<rbrakk> \<Longrightarrow> ((x \<leftrightarrow> y) \<bullet> \<Gamma>) \<turnstile> (x \<leftrightarrow> y) \<bullet> e : \<tau>"
+proof (nominal_induct \<Gamma> e \<tau> avoiding: x y rule: T.strong_induct)
+  case (T_UnitI \<Gamma>)
   then show ?case by (simp add: T.T_UnitI)
 next
-  case (T_VarI z τ Γ)
+  case (T_VarI z \<tau> \<Gamma>)
   then show ?case
     by (metis T.T_VarI T.eqvt flip_fresh_fresh no_vars_in_ty)
 next
-  case (T_AbsI x Γ τ1 e τ2)
+  case (T_AbsI x \<Gamma> \<tau>1 e \<tau>2)
   then show ?case
     by (metis T.T_AbsI T.eqvt flip_fresh_fresh no_vars_in_ty)
 next
-  case (T_AppI Γ e1 τ1 τ2 e2)
+  case (T_AppI \<Gamma> e1 \<tau>1 \<tau>2 e2)
   then show ?case using T.T_AppI by fastforce
 next
-  case (T_LetI z Γ e1 τ1 e2 τ2)
-  then have 1: "atom y ♯ (z, τ1) # Γ" by (simp add: fresh_Cons fresh_at_base(2))
+  case (T_LetI z \<Gamma> e1 \<tau>1 e2 \<tau>2)
+  then have 1: "atom y \<sharp> (z, \<tau>1) # \<Gamma>" by (simp add: fresh_Cons fresh_at_base(2))
 
-  from T_LetI have e1: "atom z ♯ (x ↔ y) ∙ e1" by (smt eq_eqvt flip_def fresh_at_base(2) fresh_eqvt swap_atom_simps(3))
-  from T_LetI have "atom z ♯ (x ↔ y) ∙ Γ" by (metis flip_def fresh_at_base(2) fresh_permute_iff swap_atom_simps(3))
-  then have 2: "atom z ♯ ((x ↔ y) ∙ Γ, (x ↔ y) ∙ e1)" using T_LetI e1 by simp
+  from T_LetI have e1: "atom z \<sharp> (x \<leftrightarrow> y) \<bullet> e1" by (smt eq_eqvt flip_def fresh_at_base(2) fresh_eqvt swap_atom_simps(3))
+  from T_LetI have "atom z \<sharp> (x \<leftrightarrow> y) \<bullet> \<Gamma>" by (metis flip_def fresh_at_base(2) fresh_permute_iff swap_atom_simps(3))
+  then have 2: "atom z \<sharp> ((x \<leftrightarrow> y) \<bullet> \<Gamma>, (x \<leftrightarrow> y) \<bullet> e1)" using T_LetI e1 by simp
 
-  from T_LetI have "(x ↔ y) ∙ ((z, τ1) # Γ) = (z, τ1)#((x ↔ y) ∙ Γ)" by (simp add: flip_fresh_fresh fresh_at_base(2))
-  then have 3: "(z, τ1) # (x ↔ y) ∙ Γ ⊢ (x ↔ y) ∙ e2 : τ2" using T_LetI(6)[OF 1, of x] by simp
+  from T_LetI have "(x \<leftrightarrow> y) \<bullet> ((z, \<tau>1) # \<Gamma>) = (z, \<tau>1)#((x \<leftrightarrow> y) \<bullet> \<Gamma>)" by (simp add: flip_fresh_fresh fresh_at_base(2))
+  then have 3: "(z, \<tau>1) # (x \<leftrightarrow> y) \<bullet> \<Gamma> \<turnstile> (x \<leftrightarrow> y) \<bullet> e2 : \<tau>2" using T_LetI(6)[OF 1, of x] by simp
 
-  show ?case using T.T_LetI[OF 2 3 T_LetI(8)[OF ‹atom y ♯ Γ›, of x]]
+  show ?case using T.T_LetI[OF 2 3 T_LetI(8)[OF \<open>atom y \<sharp> \<Gamma>\<close>, of x]]
     by (smt "1" T_LetI.hyps(1) flip_fresh_fresh fresh_Cons fresh_PairD(1) fresh_at_base(2) term.perm_simps(5))
 qed
 
 lemma T_Abs_Inv:
-  assumes a: "Γ ⊢ (λx : τ1 . e) : τ" and b: "atom x ♯ Γ"
-  shows "∃τ2. (x, τ1)#Γ ⊢ e : τ2 ∧ τ = (τ1 → τ2)"
+  assumes a: "\<Gamma> \<turnstile> (\<lambda>x : \<tau>1 . e) : \<tau>" and b: "atom x \<sharp> \<Gamma>"
+  shows "\<exists>\<tau>2. (x, \<tau>1)#\<Gamma> \<turnstile> e : \<tau>2 \<and> \<tau> = (\<tau>1 \<rightarrow> \<tau>2)"
 proof (cases rule: T.cases[OF a])
-  case (3 x' Γ' τ1' e' τ2)
+  case (3 x' \<Gamma>' \<tau>1' e' \<tau>2)
   then show ?thesis
   proof (cases "atom x' = atom x")
     case True
     then show ?thesis by (metis "3"(1) "3"(2) "3"(3) "3"(5) Abs1_eq_iff(3) atom_eq_iff term.eq_iff(2))
   next
     case False
-    then have 1: "atom x ♯ (x', τ1') # Γ'" using b by (simp add: 3 fresh_Cons) 
-    have 2: "((x' ↔ x) ∙ ((x', τ1) # Γ)) ⊢ (x' ↔ x) ∙ e' : τ2" using swap_term[OF "3"(5) 1, of x'] 3 by auto
+    then have 1: "atom x \<sharp> (x', \<tau>1') # \<Gamma>'" using b by (simp add: 3 fresh_Cons) 
+    have 2: "((x' \<leftrightarrow> x) \<bullet> ((x', \<tau>1) # \<Gamma>)) \<turnstile> (x' \<leftrightarrow> x) \<bullet> e' : \<tau>2" using swap_term[OF "3"(5) 1, of x'] 3 by auto
 
-    have 4: "(x' ↔ x) ∙ e' = e" by (metis "3"(2) Abs1_eq_iff(3) False flip_commute term.eq_iff(2))
-    have 5: "((x' ↔ x) ∙ ((x', τ1) # Γ)) = (x, τ1)#Γ" by (smt "3"(1) "3"(4) Cons_eqvt Pair_eqvt b flip_at_simps(1) flip_fresh_fresh no_vars_in_ty)
+    have 4: "(x' \<leftrightarrow> x) \<bullet> e' = e" by (metis "3"(2) Abs1_eq_iff(3) False flip_commute term.eq_iff(2))
+    have 5: "((x' \<leftrightarrow> x) \<bullet> ((x', \<tau>1) # \<Gamma>)) = (x, \<tau>1)#\<Gamma>" by (smt "3"(1) "3"(4) Cons_eqvt Pair_eqvt b flip_at_simps(1) flip_fresh_fresh no_vars_in_ty)
 
     from 2 3 4 5 show ?thesis by auto
   qed
 qed simp_all
 
 lemma T_Let_Inv:
-  assumes a: "Γ ⊢ Let x e1 e2 : τ" and b: "atom x ♯ Γ"
-  shows "∃τ1. Γ ⊢ e1 : τ1 ∧ (x, τ1)#Γ ⊢ e2 : τ"
+  assumes a: "\<Gamma> \<turnstile> Let x e1 e2 : \<tau>" and b: "atom x \<sharp> \<Gamma>"
+  shows "\<exists>\<tau>1. \<Gamma> \<turnstile> e1 : \<tau>1 \<and> (x, \<tau>1)#\<Gamma> \<turnstile> e2 : \<tau>"
 proof (cases rule: T.cases[OF a])
-  case (5 x' Γ' _ τ1 e2' τ2)
+  case (5 x' \<Gamma>' _ \<tau>1 e2' \<tau>2)
   show ?thesis
   proof (cases "atom x' = atom x")
     case True
     then show ?thesis by (metis "5"(1) "5"(2) "5"(3) "5"(5) "5"(6) Abs1_eq_iff(3) atom_eq_iff term.eq_iff(5))
   next
     case False
-    then have 1: "atom x ♯ (x', τ1) # Γ'" using b by (simp add: 5 fresh_Cons)
-    have 2: "((x' ↔ x) ∙ ((x', τ1)#Γ)) ⊢ (x' ↔ x) ∙ e2' : τ" using swap_term[OF "5"(5) 1, of x'] 5 by blast
+    then have 1: "atom x \<sharp> (x', \<tau>1) # \<Gamma>'" using b by (simp add: 5 fresh_Cons)
+    have 2: "((x' \<leftrightarrow> x) \<bullet> ((x', \<tau>1)#\<Gamma>)) \<turnstile> (x' \<leftrightarrow> x) \<bullet> e2' : \<tau>" using swap_term[OF "5"(5) 1, of x'] 5 by blast
 
-    have 3: "(x' ↔ x) ∙ e2' = e2" by (metis "5"(2) Abs1_eq_iff(3) False flip_commute term.eq_iff(5))
-    have 4: "((x' ↔ x) ∙ ((x', τ1) # Γ)) = (x, τ1)#Γ" by (smt "5"(1) "5"(4) Cons_eqvt Pair_eqvt b flip_at_simps(1) flip_fresh_fresh fresh_PairD(1) no_vars_in_ty)
+    have 3: "(x' \<leftrightarrow> x) \<bullet> e2' = e2" by (metis "5"(2) Abs1_eq_iff(3) False flip_commute term.eq_iff(5))
+    have 4: "((x' \<leftrightarrow> x) \<bullet> ((x', \<tau>1) # \<Gamma>)) = (x, \<tau>1)#\<Gamma>" by (smt "5"(1) "5"(4) Cons_eqvt Pair_eqvt b flip_at_simps(1) flip_fresh_fresh fresh_PairD(1) no_vars_in_ty)
 
     from 2 3 4 5 show ?thesis by auto
   qed
 qed simp_all
 
-lemma substitution: "⟦ (x, τ')#Γ ⊢ e : τ ; [] ⊢ v : τ' ⟧ ⟹ Γ ⊢ subst_term v x e : τ"
-proof (nominal_induct e avoiding: Γ τ v x τ' rule: term.strong_induct)
+lemma substitution: "\<lbrakk> (x, \<tau>')#\<Gamma> \<turnstile> e : \<tau> ; [] \<turnstile> v : \<tau>' \<rbrakk> \<Longrightarrow> \<Gamma> \<turnstile> subst_term v x e : \<tau>"
+proof (nominal_induct e avoiding: \<Gamma> \<tau> v x \<tau>' rule: term.strong_induct)
   case (Var y)
   then show ?case
   proof (cases "x = y")
     case True
-    then have "τ = τ'" using Var T.cases by fastforce
+    then have "\<tau> = \<tau>'" using Var T.cases by fastforce
     then show ?thesis using True Var context_invariance by fastforce
   next
     case False
@@ -174,53 +174,53 @@ proof (nominal_induct e avoiding: Γ τ v x τ' rule: term.strong_induct)
       by (metis (no_types, lifting) Rep_name_inverse atom_name_def subst_term.simps(1) isin.simps(2) singletonD supp_at_base term.fv_defs(1))
   qed
 next
-  case (Lam y σ e)
-  then obtain τ2 where P: "(y, σ)#(x, τ')#Γ ⊢ e : τ2 ∧ τ = (σ → τ2)" using T_Abs_Inv[OF Lam(7)] fresh_Cons fresh_Pair by blast
-  then have "(x, τ')#(y, σ)#Γ ⊢ e : τ2" using context_invariance ‹atom y ♯ x› by auto
+  case (Lam y \<sigma> e)
+  then obtain \<tau>2 where P: "(y, \<sigma>)#(x, \<tau>')#\<Gamma> \<turnstile> e : \<tau>2 \<and> \<tau> = (\<sigma> \<rightarrow> \<tau>2)" using T_Abs_Inv[OF Lam(7)] fresh_Cons fresh_Pair by blast
+  then have "(x, \<tau>')#(y, \<sigma>)#\<Gamma> \<turnstile> e : \<tau>2" using context_invariance \<open>atom y \<sharp> x\<close> by auto
   then show ?case using Lam T_AbsI P by simp
 next
   case (App e1 e2)
-  obtain τ1 where P: "((x, τ') # Γ ⊢ e1 : τ1 → τ) ∧ ((x, τ') # Γ ⊢ e2 : τ1)" using T.cases[OF App(3)] by fastforce
+  obtain \<tau>1 where P: "((x, \<tau>') # \<Gamma> \<turnstile> e1 : \<tau>1 \<rightarrow> \<tau>) \<and> ((x, \<tau>') # \<Gamma> \<turnstile> e2 : \<tau>1)" using T.cases[OF App(3)] by fastforce
   then show ?case using T_AppI App by fastforce
 next
   case Unit
   then show ?case using T.cases[OF Unit(1)] T_UnitI by auto
 next
   case (Let y e1 e2)
-  have "atom y ♯ e1" using Let.hyps(1) Let.hyps(4) Let.prems(1) T_Let_Inv fresh_Cons fresh_Pair fresh_term no_vars_in_ty by blast
-  then have "atom y ♯ subst_term v x e1" by (simp add: Let.hyps(3) fresh_subst_term) 
-  then have 0: "atom y ♯ (Γ, subst_term v x e1)" using Let fresh_Pair by simp
+  have "atom y \<sharp> e1" using Let.hyps(1) Let.hyps(4) Let.prems(1) T_Let_Inv fresh_Cons fresh_Pair fresh_term no_vars_in_ty by blast
+  then have "atom y \<sharp> subst_term v x e1" by (simp add: Let.hyps(3) fresh_subst_term) 
+  then have 0: "atom y \<sharp> (\<Gamma>, subst_term v x e1)" using Let fresh_Pair by simp
 
-  obtain τ1 where P: "(x, τ')#Γ ⊢ e1 : τ1 ∧ (y, τ1)#(x, τ')#Γ ⊢ e2 : τ" using T_Let_Inv[OF Let(8)] Let fresh_Cons fresh_Pair by blast
-  then have 1: "(x, τ')#(y, τ1)#Γ ⊢ e2 : τ" using context_invariance Let(4) by force
-  from P have 2: "(x, τ')#Γ ⊢ e1 : τ1" by simp
+  obtain \<tau>1 where P: "(x, \<tau>')#\<Gamma> \<turnstile> e1 : \<tau>1 \<and> (y, \<tau>1)#(x, \<tau>')#\<Gamma> \<turnstile> e2 : \<tau>" using T_Let_Inv[OF Let(8)] Let fresh_Cons fresh_Pair by blast
+  then have 1: "(x, \<tau>')#(y, \<tau>1)#\<Gamma> \<turnstile> e2 : \<tau>" using context_invariance Let(4) by force
+  from P have 2: "(x, \<tau>')#\<Gamma> \<turnstile> e1 : \<tau>1" by simp
 
-  have 3: "Γ ⊢ subst_term v x e1 : τ1" using Let(6)[OF 2 Let(9)] .
-  have 4: "(y, τ1)#Γ ⊢ subst_term v x e2 : τ" using Let(7)[OF 1 Let(9)] .
+  have 3: "\<Gamma> \<turnstile> subst_term v x e1 : \<tau>1" using Let(6)[OF 2 Let(9)] .
+  have 4: "(y, \<tau>1)#\<Gamma> \<turnstile> subst_term v x e2 : \<tau>" using Let(7)[OF 1 Let(9)] .
 
   show ?case using T_LetI[OF 0 4 3] using Let by simp
 qed
 
-theorem preservation: "⟦ [] ⊢ e : τ ; Step e e' ⟧ ⟹ [] ⊢ e' : τ"
-proof (nominal_induct "[] :: Γ" e τ arbitrary: e' rule: T.strong_induct)
+theorem preservation: "\<lbrakk> [] \<turnstile> e : \<tau> ; Step e e' \<rbrakk> \<Longrightarrow> [] \<turnstile> e' : \<tau>"
+proof (nominal_induct "[] :: \<Gamma>" e \<tau> arbitrary: e' rule: T.strong_induct)
   case T_UnitI
   then show ?case using Step.cases by fastforce
 next
-  case (T_VarI x τ)
+  case (T_VarI x \<tau>)
   then show ?case by simp
 next
-  case (T_AbsI x τ1 e τ2)
+  case (T_AbsI x \<tau>1 e \<tau>2)
   then show ?case using Step.cases by fastforce
 next
-  case (T_AppI e1 τ1 τ2 e2)
-  from ‹App e1 e2 ⟶ e'› show ?case
+  case (T_AppI e1 \<tau>1 \<tau>2 e2)
+  from \<open>App e1 e2 \<longrightarrow> e'\<close> show ?case
   proof cases
-    case (ST_BetaI x τ e)
-    then have "τ = τ1" using T_AppI.hyps(1) fun_ty_lam is_v_of_e.simps(2) term.eq_iff(2) by blast
-    then have 1: "[] ⊢ e2 : τ" using T_AppI(3) by simp
+    case (ST_BetaI x \<tau> e)
+    then have "\<tau> = \<tau>1" using T_AppI.hyps(1) fun_ty_lam is_v_of_e.simps(2) term.eq_iff(2) by blast
+    then have 1: "[] \<turnstile> e2 : \<tau>" using T_AppI(3) by simp
 
-    have "[] ⊢ λ x : τ . e : τ1 → τ2" using T_AppI ST_BetaI by blast
-    then have 2: "[(x, τ)] ⊢ e : τ2" using T_Abs_Inv fresh_Nil by fastforce
+    have "[] \<turnstile> \<lambda> x : \<tau> . e : \<tau>1 \<rightarrow> \<tau>2" using T_AppI ST_BetaI by blast
+    then have 2: "[(x, \<tau>)] \<turnstile> e : \<tau>2" using T_Abs_Inv fresh_Nil by fastforce
 
     show ?thesis using substitution[OF 2 1] ST_BetaI by simp
   next
@@ -231,8 +231,8 @@ next
     then show ?thesis using T_AppI T.T_AppI by blast
   qed
 next
-  case (T_LetI x e1 τ1 e2 τ2)
-  from ‹Let x e1 e2 ⟶ e'› show ?case
+  case (T_LetI x e1 \<tau>1 e2 \<tau>2)
+  from \<open>Let x e1 e2 \<longrightarrow> e'\<close> show ?case
   proof cases
     case (ST_SubstI y e)
 
@@ -242,9 +242,9 @@ next
       then show ?thesis by (metis Abs1_eq(3) T_LetI.hyps(3) T_LetI.hyps(4) atom_eq_iff local.ST_SubstI(1) local.ST_SubstI(2) substitution)
     next
       case False
-      then have 1: "atom y ♯ [(x, τ1)]" by (simp add: fresh_Cons fresh_Nil)
-      have "(x ↔ y) ∙ e2 = e" by (metis Abs1_eq_iff'(3) False flip_commute local.ST_SubstI(1))
-      then have "[(y, τ1)] ⊢ e : τ2" using swap_term[OF T_LetI(3) 1, of x] by (simp add: flip_fresh_fresh)
+      then have 1: "atom y \<sharp> [(x, \<tau>1)]" by (simp add: fresh_Cons fresh_Nil)
+      have "(x \<leftrightarrow> y) \<bullet> e2 = e" by (metis Abs1_eq_iff'(3) False flip_commute local.ST_SubstI(1))
+      then have "[(y, \<tau>1)] \<turnstile> e : \<tau>2" using swap_term[OF T_LetI(3) 1, of x] by (simp add: flip_fresh_fresh)
       then show ?thesis using T_LetI ST_SubstI substitution by auto
     qed
   next
@@ -253,18 +253,18 @@ next
   qed
 qed
 
-definition stuck :: "term ⇒ bool" where
-  "stuck e ≡ ¬(is_v_of_e e ∨ (∃e'. Step e e'))"
+definition stuck :: "term \<Rightarrow> bool" where
+  "stuck e \<equiv> \<not>(is_v_of_e e \<or> (\<exists>e'. Step e e'))"
 
-inductive Steps :: "term ⇒ term ⇒ bool" (infix "⟶*" 70) where
+inductive Steps :: "term \<Rightarrow> term \<Rightarrow> bool" (infix "\<longrightarrow>*" 70) where
   refl: "Steps e e"
-| trans: "⟦ Steps e1 e2 ; Step e2 e3 ⟧ ⟹ Steps e1 e3"
+| trans: "\<lbrakk> Steps e1 e2 ; Step e2 e3 \<rbrakk> \<Longrightarrow> Steps e1 e3"
 
-lemma multi_preservation: "⟦ e ⟶* e' ; [] ⊢ e : τ ⟧ ⟹ [] ⊢ e' : τ"
+lemma multi_preservation: "\<lbrakk> e \<longrightarrow>* e' ; [] \<turnstile> e : \<tau> \<rbrakk> \<Longrightarrow> [] \<turnstile> e' : \<tau>"
   apply (induction e e' rule: Steps.induct)
   using preservation by blast+
 
-corollary soundness: "⟦ [] ⊢ e : τ ; e ⟶* e' ⟧ ⟹ ¬(stuck e')"
+corollary soundness: "\<lbrakk> [] \<turnstile> e : \<tau> ; e \<longrightarrow>* e' \<rbrakk> \<Longrightarrow> \<not>(stuck e')"
   unfolding stuck_def
   using progress multi_preservation by blast
 
