Dockerfile
@@ -1,0 +1,15 @@
+FROM makarius/isabelle:Isabelle2020
+
+RUN for t in Nominal2 FinFun; do \
+        curl https://www.isa-afp.org/release/afp-$t-current.tar.gz -o $t.tar.gz ; \
+        cd Isabelle/src/ ; \
+        tar -xzf ../../$t.tar.gz ; \
+        cd .. ; \
+        echo "src/$t" >> ROOTS ; \
+        cd .. ; \
+        rm $t.tar.gz ; \
+    done
+
+RUN ./Isabelle/bin/isabelle build -o system_heaps -b Nominal2
+
+COPY ROOT Defs.thy Soundness.thy ./
