ROOT
@@ -1,0 +1,4 @@
+session Lambda = HOL + sessions "HOL-Eisbach" Nominal2
+theories
+    Defs
+    Soundness
